term.v
@@ -3,24 +3,59 @@ From iris.heap_lang Require Import notation.
 From iris.heap_lang Require Import primitive_laws.
 From crypto Require Import lib basic symbols.
 
+Inductive key_type := KSym | KAEnc | KADec.
+
+Definition int_of_key_type kt : Z :=
+  match kt with
+  | KSym => 0
+  | KAEnc => 1
+  | KADec => 2
+  end.
+
+Definition key_type_of_int (n : Z) :=
+  match n with
+  | 0%Z => KSym
+  | 1%Z => KAEnc
+  | _ => KADec
+  end.
+
+Canonical key_typeO := leibnizO key_type.
+
+Instance key_type_eq_dec : EqDecision key_type.
+Proof.
+refine (
+  fun kt1 kt2 =>
+    match kt1, kt2 with
+    | KSym, KSym => left _
+    | KAEnc, KAEnc => left _
+    | KADec, KADec => left _
+    | _, _ => right _
+    end); congruence.
+Defined.
+
+Instance int_of_key_typeK : Cancel (=) key_type_of_int int_of_key_type.
+Proof. by case. Qed.
+
+Instance int_of_key_type_inj : Inj (=) (=) int_of_key_type.
+Proof. by apply (@cancel_inj _ _ _ key_type_of_int); apply _. Qed.
+
+Instance int_of_key_type_countable : Countable key_type.
+Proof. apply (inj_countable' _ _ int_of_key_typeK). Qed.
+
 Inductive term  :=
 | TInt of Z
 | TPair of term & term
 | TNonce of loc
-| TAKey of loc & bool
-| TAEnc of loc & term
-| TSKey of loc
-| TSEnc of loc & term.
+| TKey of key_type & loc
+| TEnc of bool & loc & term.
 
 Canonical termO := leibnizO term.
 
 Notation TInt_tag := 0%Z.
 Notation TPair_tag := 1%Z.
 Notation TNonce_tag := 2%Z.
-Notation TAKey_tag := 3%Z.
-Notation TAEnc_tag := 4%Z.
-Notation TSKey_tag := 5%Z.
-Notation TSEnc_tag := 6%Z.
+Notation TKey_tag := 3%Z.
+Notation TEnc_tag := 4%Z.
 
 Global Instance term_eq_dec : EqDecision term.
 Proof.
@@ -33,14 +68,10 @@ refine (
       cast_if_and (decide (t11 = t21)) (decide (t12 = t22))
     | TNonce l1, TNonce l2 =>
       cast_if (decide (l1 = l2))
-    | TAKey l1 b1, TAKey l2 b2 =>
-      cast_if_and (decide (l1 = l2)) (decide (b1 = b2))
-    | TAEnc l1 t1, TAEnc l2 t2 =>
-      cast_if_and (decide (l1 = l2)) (decide (t1 = t2))
-    | TSKey l1, TSKey l2 =>
-      cast_if (decide (l1 = l2))
-    | TSEnc l1 t1, TSEnc l2 t2 =>
-      cast_if_and (decide (l1 = l2)) (decide (t1 = t2))
+    | TKey kt1 l1, TKey kt2 l2 =>
+      cast_if_and (decide (kt1 = kt2)) (decide (l1 = l2))
+    | TEnc asym1 l1 t1, TEnc asym2 l2 t2 =>
+      cast_if_and3 (decide (asym1 = asym2)) (decide (l1 = l2)) (decide (t1 = t2))
     | _, _ => right _
     end); clear go; abstract intuition congruence.
 Defined.
@@ -50,10 +81,8 @@ Fixpoint val_of_term_rec t : val :=
   | TInt n => (#TInt_tag, #n)
   | TPair t1 t2 => (#TPair_tag, (val_of_term_rec t1, val_of_term_rec t2))%V
   | TNonce l => (#TNonce_tag, #l)%V
-  | TAKey l b => (#TAKey_tag, (#l, #b))%V
-  | TAEnc l t => (#TAEnc_tag, (#l, val_of_term_rec t))%V
-  | TSKey l => (#TSKey_tag, #l)%V
-  | TSEnc l t => (#TSEnc_tag, (#l, val_of_term_rec t))
+  | TKey kt l => (#TKey_tag, (#(int_of_key_type kt), #l))%V
+  | TEnc b l t => (#TEnc_tag, (#b, #l, val_of_term_rec t))%V
   end.
 
 Definition val_of_term := locked val_of_term_rec.
@@ -70,19 +99,18 @@ Fixpoint term_of_val v : term :=
     TPair (term_of_val v1) (term_of_val v2)
   | PairV (# (LitInt TNonce_tag)) (# (LitLoc l)) =>
     TNonce l
-  | PairV #(LitInt TAKey_tag) (PairV #(LitLoc l) #(LitBool b)) =>
-    TAKey l b
-  | PairV #(LitInt TAEnc_tag) (PairV #(LitLoc l) v) =>
-    TAEnc l (term_of_val v)
-  | PairV (# (LitInt TSKey_tag)) (# (LitLoc l)) =>
-    TSKey l
-  | PairV (# (LitInt TSEnc_tag)) (PairV (# (LitLoc l)) v) =>
-    TSEnc l (term_of_val v)
+  | PairV #(LitInt TKey_tag) (#(LitInt n), #(LitLoc l)) =>
+    TKey (key_type_of_int n) l
+  | PairV #(LitInt TEnc_tag) (#(LitBool b), #(LitLoc l), v) =>
+    TEnc b l (term_of_val v)
   | _ => TInt 0
   end.
 
 Global Instance val_of_termK : Cancel (=) term_of_val val_of_term.
-Proof. rewrite val_of_termE; elim=> //= *; congruence. Qed.
+Proof.
+rewrite val_of_termE; elim=> //= *; try by congruence.
+by rewrite cancel.
+Qed.
 
 Global Instance val_of_term_inj : Inj (=) (=) val_of_term.
 Proof.
